Add space for inode allocation to data layout

src/Dafny/examples/fs/kinds.dfy
@@ -1,4 +1,5 @@
 include "../../jrnl/jrnl.s.dfy"
+include "../../nonlin/roundup.dfy"
 
 module FsKinds {
   import Arith
@@ -6,12 +7,14 @@ module FsKinds {
   import opened JrnlTypes
   import opened JrnlSpec
   import opened Kinds
+  import Round
 
   type Ino = uint64
 
   datatype Super = Super(inode_blocks: nat, data_bitmaps: nat)
   {
     const num_inodes: nat := 32 * inode_blocks
+    const inode_bitmaps: nat := Round.div_roundup_alt(num_inodes, 4096*8)
     const num_data_blocks: nat := data_bitmaps * (4096*8)
 
     static const zero := Super(0, 0)
@@ -23,20 +26,24 @@ module FsKinds {
       && disk_size < U64.MAX
     }
 
-    // prior to data, disk layout is:
-    //
-    // 513 blocks reserved for the journal
-    // inode_blocks hold the inodes
-    // data_bitmaps are allocators for the data blocks
-    //
-    // these are followed by num_data_blocks data blocks
-    const data_start: nat := 513 + inode_blocks + data_bitmaps
-
     // NOTE(tej): hack because otherwise non-linear arithmetic in num_data_blocks confuses Dafny and it doesn't know the sum is still a nat
     static function method add_nats(n1: nat, n2: nat): nat
     {
       n1 + n2
     }
+
+    // prior to data, disk layout is:
+    //
+    // 513 blocks reserved for the journal
+    // inode_blocks hold the inodes
+    // data_bitmaps are allocators for the data blocks
+    // inode_bitmaps are allocators for inodes
+    //
+    // these are followed by num_data_blocks data blocks
+    const data_bitmap_start: nat := 513 + inode_blocks
+    const inode_bitmap_start: nat := data_bitmap_start + data_bitmaps
+    const data_start: nat := add_nats(inode_bitmap_start, inode_bitmaps)
+
     const disk_size: nat := add_nats(data_start, num_data_blocks)
   }
 
@@ -60,7 +67,7 @@ module FsKinds {
     513 + ino / 32
   }
 
-  predicate method InodeBlk?(bn: Blkno)
+  predicate InodeBlk?(bn: Blkno)
   {
     513 <= bn as nat < 513 + super.inode_blocks
   }
@@ -76,17 +83,17 @@ module FsKinds {
   function method DataAllocBlk(bn: Blkno): (bn':Blkno)
     ensures blkno_ok(bn) ==> DataAllocBlk?(bn')
   {
-    var bn' := 513 + super.inode_blocks as uint64 + bn / (4096*8);
+    var bn' := super.data_bitmap_start as uint64 + bn / (4096*8);
     if bn as nat < super.data_bitmaps*(4096*8) then (
       Arith.div_incr(bn as nat, super.data_bitmaps, 4096*8);
       bn'
     ) else bn'
   }
 
-  predicate method DataAllocBlk?(bn: Blkno)
+  predicate DataAllocBlk?(bn: Blkno)
   {
-    var start := 513 + super.inode_blocks;
-    start <= bn as nat < start + super.data_bitmaps as nat
+    var start := super.data_bitmap_start;
+    start <= bn as nat < start + super.data_bitmaps
   }
 
   lemma DataAllocBlk?_correct(bn: Blkno)
@@ -97,6 +104,22 @@ module FsKinds {
       assert blkno_ok(bn');
       assert DataAllocBlk(bn') == bn;
     }
+  }
+
+  function method InodeAllocBlk(ino: Ino): (bn: Blkno)
+    ensures ino_ok(ino) ==> InodeAllocBlk?(bn)
+  {
+    var bn := super.inode_bitmap_start as uint64 + ino / (4096*8);
+    if ino < super.num_inodes as uint64 then (
+      Arith.div_incr(ino as nat, super.inode_bitmaps, 4096*8);
+      bn
+    ) else bn
+  }
+
+  predicate InodeAllocBlk?(bn: Blkno)
+  {
+    var start := super.inode_bitmap_start;
+    start <= bn as nat < start + super.inode_bitmaps
   }
 
   function method {:opaque} InodeAddr(ino: Ino): (a:Addr)
@@ -115,12 +138,17 @@ module FsKinds {
     reveal_addrsForKinds();
     Addr(ino_blk, ino_off*128*8)
   }
-  function method DataBitAddr(bn: uint64): Addr
+  function method DataBitAddr(bn: Blkno): Addr
     requires blkno_ok(bn)
   {
     Addr(DataAllocBlk(bn), bn % (4096*8))
   }
-  function method {:opaque} DataBlk(bn: uint64): (a:Addr)
+  function method InodeBitAddr(ino: Ino): Addr
+    requires ino_ok(ino)
+  {
+    Addr(InodeAllocBlk(ino), ino % (4096*8))
+  }
+  function method {:opaque} DataBlk(bn: Blkno): (a:Addr)
     requires blkno_ok(bn)
     ensures a in addrsForKinds(fs_kinds)
   {
@@ -129,6 +157,10 @@ module FsKinds {
     Arith.zero_mod(4096*8);
     reveal_addrsForKinds();
     Addr(super.data_start as uint64+bn, 0)
+  }
+  predicate DataBlk?(bn: uint64)
+  {
+    super.data_start <= bn as nat
   }
 
   lemma InodeAddr_inj()
@@ -141,6 +173,7 @@ module FsKinds {
   lemma InodeAddr_disjoint(ino: Ino)
     requires ino_ok(ino)
     ensures forall bn': Blkno | blkno_ok(bn') :: InodeAddr(ino) != DataBitAddr(bn')
+    ensures forall ino' : Ino | ino_ok(ino') :: InodeAddr(ino) != InodeBitAddr(ino')
     ensures forall bn': Blkno | blkno_ok(bn') :: InodeAddr(ino) != DataBlk(bn')
   {
     reveal_DataBlk();
@@ -156,6 +189,7 @@ module FsKinds {
   lemma DataBitAddr_disjoint(bn: Blkno)
     requires blkno_ok(bn)
     ensures forall ino': Ino | ino_ok(ino') :: DataBitAddr(bn) != InodeAddr(ino')
+    ensures forall ino': Ino | ino_ok(ino') :: DataBitAddr(bn) != InodeBitAddr(ino')
     ensures forall bn': Blkno | blkno_ok(bn') :: DataBitAddr(bn) != DataBlk(bn')
   {
     reveal_DataBlk();
@@ -165,20 +199,24 @@ module FsKinds {
   lemma DataBlk_disjoint(bn: Blkno)
     requires blkno_ok(bn)
     ensures forall ino': Ino | ino_ok(ino') :: DataBlk(bn) != InodeAddr(ino')
+    ensures forall ino': Ino | ino_ok(ino') :: DataBlk(bn) != InodeBitAddr(ino')
     ensures forall bn': Ino | blkno_ok(bn') :: DataBlk(bn) != DataBitAddr(bn')
   {
     reveal_DataBlk();
     reveal_InodeAddr();
   }
 
-  const fs_kinds: map<Blkno, Kind> :=
+  ghost const fs_kinds: map<Blkno, Kind> :=
     map blkno: Blkno |
       513 <= blkno as nat < super.disk_size
       :: (if InodeBlk?(blkno)
-      then KindInode
-      else if DataAllocBlk?(blkno)
-        then KindBit
-        else KindBlock) as Kind
+          then KindInode
+        else if DataAllocBlk?(blkno)
+          then KindBit
+        else if InodeAllocBlk?(blkno)
+          then KindBit
+        else (assert DataBlk?(blkno); KindBlock)
+      ) as Kind
 
   lemma fs_kinds_valid()
     ensures kindsValid(fs_kinds)
